C-verifier/src/Midend-IVL/Isabelle-UTP-Extended/utp/utp_sp.thy
@@ -15,7 +15,7 @@ definition sp_upred :: "'\<alpha> cond \<Rightarrow> ('\<alpha>, '\<beta>) rel \
 
 adhoc_overloading
   usp sp_upred
-  
+
 declare sp_upred_def [upred_defs]
 
 lemma sp_false [sp]: "p sp false = false"
